IMLTT/typed/proofs/Recursor.lean
@@ -33,8 +33,9 @@ theorem judgment_recursor :
     (a : Γ ctx), motive_1 Γ a → motive_2 Γ 𝒰 (IsType.univ_form a))
   → (IsTypeUnivElim : ∀ {n : Nat} {Γ : Ctx n} {A : Tm n} (a : Γ ⊢ A ∶ 𝒰),
     motive_3 Γ A 𝒰 a → motive_2 Γ A (IsType.univ_elim a))
-  → (HasTypeVar : ∀ {x : Nat} {Γ : Ctx x} {A : Tm x} 
-    (a : Γ ⊢ A type), motive_2 Γ A a → motive_3 (Γ ⬝ A) v(0) (weaken (.shift .id) A) (HasType.var a))
+  → (HasTypeVar : ∀ {x : Nat} {Γ : Ctx x} {A : Tm x} {A' : Tm (x + 1)}
+    (a : Γ ⊢ A type) (a1 : A' = weaken (.shift .id) A),
+    motive_2 Γ A a → motive_3 (Γ ⬝ A) v(0) A' (HasType.var a a1))
   → (HasTypeUnitIntro : ∀ {n : Nat} {Γ : Ctx n}
     (a : Γ ctx), motive_1 Γ a → motive_3 Γ ⋆ 𝟙 (HasType.unit_intro a))
   → (HasTypePiIntro : ∀ {n : Nat} {Γ : Ctx n} {A : Tm n} {b B : Tm (n + 1)} 
@@ -61,37 +62,39 @@ theorem judgment_recursor :
     (a_1 : Γ ⊢ A ∶ 𝒰) (a_2 : Γ ⊢ a ∶ A) (a_3 : Γ ⊢ a' ∶ A),
     motive_3 Γ A 𝒰 a_1 → motive_3 Γ a A a_2 → motive_3 Γ a' A a_3 
     → motive_3 Γ (.iden A a a') 𝒰 (HasType.univ_iden a_1 a_2 a_3))
-  → (HasTypeUnitElim : ∀ {n : Nat} {Γ : Ctx n} {A : Tm (n + 1)} {a b : Tm n} 
-    (a_1 : (Γ ⬝ 𝟙) ⊢ A type) (a_2 : Γ ⊢ a ∶ substitute_zero A ⋆) (a_3 : Γ ⊢ b ∶ 𝟙),
+  → (HasTypeUnitElim : ∀ {n : Nat} {Γ : Ctx n} {A : Tm (n + 1)} {a b : Tm n} {S : Tm n}
+    (a_1 : (Γ ⬝ 𝟙) ⊢ A type) (a_2 : Γ ⊢ a ∶ substitute_zero A ⋆) (a_3 : Γ ⊢ b ∶ 𝟙)
+    (a_4 : S = substitute_zero A b),
     motive_2 (Γ ⬝ 𝟙) A a_1 → motive_3 Γ a (substitute_zero A ⋆) a_2 → motive_3 Γ b 𝟙 a_3 
-    → motive_3 Γ (.indUnit A b a) (substitute_zero A b) (HasType.unit_elim a_1 a_2 a_3))
-  → (HasTypeEmptyElim : ∀ {n : Nat} {Γ : Ctx n} {A : Tm (n + 1)} {b : Tm n} 
-    (a : (Γ ⬝ 𝟘) ⊢ A type) (a_1 : Γ ⊢ b ∶ 𝟘), 
-    motive_2 (Γ ⬝ 𝟘) A a → motive_3 Γ b 𝟘 a_1 
-    → motive_3 Γ (.indEmpty A b) (substitute_zero A b) (HasType.empty_elim a a_1))
-  → (HasTypePiElim : ∀ {n : Nat} {Γ : Ctx n} {f A : Tm n} {B : Tm (n + 1)} {a : Tm n} 
-    (a_1 : Γ ⊢ f ∶ (.pi A B)) (a_2 : Γ ⊢ a ∶ A),
+    → motive_3 Γ (.indUnit A b a) S (HasType.unit_elim a_1 a_2 a_3 a_4))
+  → (HasTypeEmptyElim : ∀ {n : Nat} {Γ : Ctx n} {A : Tm (n + 1)} {b : Tm n} {S : Tm n}
+    (a : (Γ ⬝ 𝟘) ⊢ A type) (a_1 : Γ ⊢ b ∶ 𝟘) (a_2 : S = substitute_zero A b),
+    motive_2 (Γ ⬝ 𝟘) A a → motive_3 Γ b 𝟘 a_1
+    → motive_3 Γ (.indEmpty A b) S (HasType.empty_elim a a_1 a_2))
+  → (HasTypePiElim : ∀ {n : Nat} {Γ : Ctx n} {f A : Tm n} {B : Tm (n + 1)} {a : Tm n} {S : Tm n}
+    (a_1 : Γ ⊢ f ∶ (.pi A B)) (a_2 : Γ ⊢ a ∶ A) (a_3 : S = substitute_zero B a),
     motive_3 Γ f (.pi A B) a_1 → motive_3 Γ a A a_2 
-    → motive_3 Γ (.app f a) (substitute_zero B a) (HasType.pi_elim a_1 a_2))
-  → (HasTypeSigmaElim : ∀ {n : Nat} {Γ : Ctx n} {A : Tm n} {B : Tm (n + 1)} {p : Tm n} 
+    → motive_3 Γ (.app f a) S (HasType.pi_elim a_1 a_2 a_3))
+  → (HasTypeSigmaElim : ∀ {n : Nat} {Γ : Ctx n} {A : Tm n} {B : Tm (n + 1)} {p : Tm n} {S : Tm n}
     {C : Tm (n + 1)} {c : Tm (n + 1 + 1)}
     (a_1 : Γ ⊢ p ∶ (.sigma A B)) (a_2 : (Γ ⬝ (.sigma A B)) ⊢ C type)
-    (a_3 : (Γ ⬝ A ⬝ B) ⊢ c ∶ (substitute (Subst.weak (.shift (.shift .id)), 
-      (.pairSigma v(1) v(0))) C)),
+    (a_3 : (Γ ⬝ A ⬝ B) ⊢ c ∶ (substitute (Subst.weak (.shift (.shift .id)),
+      (.pairSigma v(1) v(0))) C))
+    (a_4 : S = substitute_zero C p),
     motive_3 Γ p (.sigma A B) a_1 → motive_2 (Γ ⬝ (.sigma A B)) C a_2
     → motive_3 (Γ ⬝ A ⬝ B) c
       (substitute (Subst.weak (.shift (.shift .id)), (.pairSigma v(1) v(0))) C) a_3
-    → motive_3 Γ (.indSigma A B C c p) (substitute_zero C p) (HasType.sigma_elim a_1 a_2 a_3) )
+    → motive_3 Γ (.indSigma A B C c p) S (HasType.sigma_elim a_1 a_2 a_3 a_4))
   → (HasTypeIdenElim : ∀ {n : Nat} {Γ : Ctx n} {A : Tm n} {B : Tm (n + 1 + 1 + 1)} {b : Tm n} 
-    {a a' p : Tm n}
+    {a a' p : Tm n} {S : Tm n}
     (a_1 : (Γ ⬝ A ⬝ (weaken Weak.id.shift A) ⬝ (weaken Weak.id.shift.shift A).iden v(1) v(0)) ⊢ B type)
     (a_2 : Γ ⊢ b ∶ substitute (Subst.weak .id, a, a, .refl A a) B)
-    (a_4 : Γ ⊢ p ∶ A.iden a a'),
+    (a_4 : Γ ⊢ p ∶ A.iden a a')
+    (a_5 : S = (substitute (Subst.weak Weak.id, a, a', p) B)),
     motive_2 (Γ ⬝ A ⬝ weaken Weak.id.shift A ⬝ (weaken Weak.id.shift.shift A).iden v(1) v(0)) B a_1 
     → motive_3 Γ b (substitute (Subst.weak .id, a, a, .refl A a) B) a_2
     → motive_3 Γ p (A.iden a a') a_4 
-    → motive_3 Γ (A.j B b a a' p) (substitute (Subst.weak Weak.id, a, a', p) B) 
-      (HasType.iden_elim a_1 a_2 a_4))
+    → motive_3 Γ (A.j B b a a' p) S (HasType.iden_elim a_1 a_2 a_4 a_5))
   → (HasTypeTyConv : ∀ {n : Nat} {Γ : Ctx n} {a A B : Tm n}
     (a_1 : Γ ⊢ a ∶ A) (a_2 : Γ ⊢ A ≡ B type), 
     motive_3 Γ a A a_1 → motive_4 Γ A B a_2 
@@ -116,80 +119,85 @@ theorem judgment_recursor :
     (a : Γ ctx), motive_1 Γ a → motive_4 Γ 𝒰 𝒰 (IsEqualType.univ_form_eq a))
   → (IsEqualTypeUnivElimEq : ∀ {n : Nat} {Γ : Ctx n} {A A' : Tm n} 
     (a : Γ ⊢ A ≡ A' ∶ 𝒰), motive_5 Γ A A' 𝒰 a → motive_4 Γ A A' (IsEqualType.univ_elim_eq a))
-  → (IsEqualTermVarEq : ∀ {x : Nat} {Γ : Ctx x} {A : Tm x} 
-    (a : Γ ⊢ A type), motive_2 Γ A a 
-    → motive_5 (Γ ⬝ A) v(0) v(0) (weaken Weak.id.shift A) (IsEqualTerm.var_eq a))
-  → (IsEqualTermUnitComp : ∀ {n : Nat} {Γ : Ctx n} {A : Tm (n + 1)} {a : Tm n} 
-    (a_1 : (Γ ⬝ 𝟙) ⊢ A type) (a_2 : Γ ⊢ a ∶ substitute_zero A ⋆),
+  → (IsEqualTermVarEq : ∀ {x : Nat} {Γ : Ctx x} {A : Tm x} {S : Tm (x + 1)}
+    (a : Γ ⊢ A type) (a_1 : S = (weaken Weak.id.shift A)), motive_2 Γ A a
+    → motive_5 (Γ ⬝ A) v(0) v(0) S (IsEqualTerm.var_eq a a_1))
+  → (IsEqualTermUnitComp : ∀ {n : Nat} {Γ : Ctx n} {A : Tm (n + 1)} {a : Tm n} {S : Tm n}
+    (a_1 : (Γ ⬝ 𝟙) ⊢ A type) (a_2 : Γ ⊢ a ∶ substitute_zero A ⋆) (a_3 : S = substitute_zero A ⋆),
     motive_2 (Γ ⬝ 𝟙) A a_1 → motive_3 Γ a (substitute_zero A ⋆) a_2 
-    → motive_5 Γ (A.indUnit ⋆ a) a (substitute_zero A ⋆) (IsEqualTerm.unit_comp a_1 a_2))
-  → (IsEqualTermPiComp : ∀ {n : Nat} {Γ : Ctx n} {A : Tm n} {b B : Tm (n + 1)} {a : Tm n} 
-    (a_1 : (Γ ⬝ A) ⊢ b ∶ B) (a_2 : Γ ⊢ a ∶ A), motive_3 (Γ ⬝ A) b B a_1 → motive_3 Γ a A a_2 
-    → motive_5 Γ ((A.lam b).app a) (substitute_zero b a) (substitute_zero B a) 
-      (IsEqualTerm.pi_comp a_1 a_2))
-  → (IsEqualTermSigmaComp : ∀ {n : Nat} {Γ : Ctx n} {a A b : Tm n} {B C : Tm (n + 1)} 
+    → motive_5 Γ (A.indUnit ⋆ a) a S (IsEqualTerm.unit_comp a_1 a_2 a_3))
+  → (IsEqualTermPiComp : ∀ {n : Nat} {Γ : Ctx n} {A : Tm n} {b B : Tm (n + 1)} {a : Tm n} {s S : Tm n}
+    (a_1 : (Γ ⬝ A) ⊢ b ∶ B) (a_2 : Γ ⊢ a ∶ A)
+    (a_3 : s = substitute_zero b a) (a_4 : S = substitute_zero B a),
+    motive_3 (Γ ⬝ A) b B a_1 → motive_3 Γ a A a_2 
+    → motive_5 Γ ((A.lam b).app a) s S (IsEqualTerm.pi_comp a_1 a_2 a_3 a_4))
+  → (IsEqualTermSigmaComp : ∀ {n : Nat} {Γ : Ctx n} {a A b : Tm n} {B C : Tm (n + 1)} {s S : Tm n}
     {c : Tm (n + 1 + 1)} (a_1 : Γ ⊢ a ∶ A)
     (a_2 : Γ ⊢ b ∶ substitute_zero B a) (a_3 : (Γ ⬝ A.sigma B) ⊢ C type)
-    (a_4 : (Γ ⬝ A ⬝ B) ⊢ c ∶ substitute (Subst.weak Weak.id.shift.shift, v(1).pairSigma v(0)) C),
+    (a_4 : (Γ ⬝ A ⬝ B) ⊢ c ∶ substitute (Subst.weak Weak.id.shift.shift, v(1).pairSigma v(0)) C)
+    (a_5 : s = (substitute (Subst.weak Weak.id, a, b) c))
+    (a_6 : S = (substitute_zero C (a.pairSigma b))),
     motive_3 Γ a A a_1 → motive_3 Γ b (substitute_zero B a) a_2 → motive_2 (Γ ⬝ A.sigma B) C a_3 
-    → motive_3 (Γ ⬝ A ⬝ B) c (substitute (Subst.weak Weak.id.shift.shift, v(1).pairSigma v(0)) C) a_4 
-    → motive_5 Γ (A.indSigma B C c (a.pairSigma b)) (substitute (Subst.weak Weak.id, a, b) c)
-      (substitute_zero C (a.pairSigma b)) (IsEqualTerm.sigma_comp a_1 a_2 a_3 a_4))
-  → (IsEqualTermIdenComp : ∀ {n : Nat} {Γ : Ctx n} {A : Tm n} {B : Tm (n + 1 + 1 + 1)} 
-    {b : Tm n} {a : Tm n}
+    → motive_3 (Γ ⬝ A ⬝ B) c (substitute (Subst.weak Weak.id.shift.shift, v(1).pairSigma v(0)) C) a_4
+    → motive_5 Γ (A.indSigma B C c (a.pairSigma b)) s S (IsEqualTerm.sigma_comp a_1 a_2 a_3 a_4 a_5 a_6))
+  → (IsEqualTermIdenComp : ∀ {n : Nat} {Γ : Ctx n} {A : Tm n} {B : Tm (n + 1 + 1 + 1)}
+    {b : Tm n} {a : Tm n} {S : Tm n}
     (a_1 : (Γ ⬝ A ⬝ (weaken Weak.id.shift A) ⬝ (weaken Weak.id.shift.shift A).iden v(1) v(0)) ⊢ B type)
     (a_2 : Γ ⊢ b ∶ (substitute (Subst.weak Weak.id, a, a, .refl A a) B))
-    (a_3 : Γ ⊢ a ∶ A),
-    motive_2 (Γ ⬝ A ⬝ (weaken Weak.id.shift A) ⬝ (weaken Weak.id.shift.shift A).iden v(1) v(0)) B a_1 
+    (a_3 : Γ ⊢ a ∶ A)
+    (a_4 : S = (substitute (Subst.weak Weak.id, a, a, A.refl a) B)),
+    motive_2 (Γ ⬝ A ⬝ (weaken Weak.id.shift A) ⬝ (weaken Weak.id.shift.shift A).iden v(1) v(0)) B a_1
     → motive_3 Γ b (substitute (Subst.weak Weak.id, a, a, .refl A a) B) a_2
     → motive_3 Γ a A a_3
-    → motive_5 Γ (A.j B b a a (A.refl a)) b
-      (substitute (Subst.weak Weak.id, a, a, A.refl a) B) (IsEqualTerm.iden_comp a_1 a_2 a_3))
+    → motive_5 Γ (A.j B b a a (A.refl a)) b S (IsEqualTerm.iden_comp a_1 a_2 a_3 a_4))
   → (IsEqualTermUnitIntroEq : ∀ {n : Nat} {Γ : Ctx n} 
     (a : Γ ctx), motive_1 Γ a → motive_5 Γ ⋆ ⋆ 𝟙 (IsEqualTerm.unit_intro_eq a))
-  → (IsEqualTermUnitElimEq : ∀ {n : Nat} {Γ : Ctx n} {A A' : Tm (n + 1)} {a a' b b' : Tm n} 
-    (a_1 : (Γ ⬝ 𝟙) ⊢ A ≡ A' type) (a_2 : Γ ⊢ a ≡ a' ∶ substitute_zero A ⋆) (a_3 : Γ ⊢ b ≡ b' ∶ 𝟙),
+  → (IsEqualTermUnitElimEq : ∀ {n : Nat} {Γ : Ctx n} {A A' : Tm (n + 1)} {a a' b b' : Tm n} {S : Tm n}
+    (a_1 : (Γ ⬝ 𝟙) ⊢ A ≡ A' type) (a_2 : Γ ⊢ a ≡ a' ∶ substitute_zero A ⋆) (a_3 : Γ ⊢ b ≡ b' ∶ 𝟙)
+    (a_4 : S = (substitute_zero A b)),
     motive_4 (Γ ⬝ 𝟙) A A' a_1 → motive_5 Γ a a' (substitute_zero A ⋆) a_2 → motive_5 Γ b b' 𝟙 a_3 
-    → motive_5 Γ (A.indUnit b a) (A'.indUnit b' a') (substitute_zero A b) 
-      (IsEqualTerm.unit_elim_eq a_1 a_2 a_3))
-  → (IsEqualTermEmptyElimEq : ∀ {n : Nat} {Γ : Ctx n} {A A' : Tm (n + 1)} {b b' : Tm n} 
-    (a : (Γ ⬝ 𝟘) ⊢ A ≡ A' type) (a_1 : Γ ⊢ b ≡ b' ∶ 𝟘), motive_4 (Γ ⬝ 𝟘) A A' a → motive_5 Γ b b' 𝟘 a_1 
-    → motive_5 Γ (A.indEmpty b) (A'.indEmpty b') (substitute_zero A b) (IsEqualTerm.empty_elim_eq a a_1))
+    → motive_5 Γ (A.indUnit b a) (A'.indUnit b' a') S (IsEqualTerm.unit_elim_eq a_1 a_2 a_3 a_4))
+  → (IsEqualTermEmptyElimEq : ∀ {n : Nat} {Γ : Ctx n} {A A' : Tm (n + 1)} {b b' : Tm n} {S : Tm n}
+    (a : (Γ ⬝ 𝟘) ⊢ A ≡ A' type) (a_1 : Γ ⊢ b ≡ b' ∶ 𝟘) (a_2 : S = substitute_zero A b),
+    motive_4 (Γ ⬝ 𝟘) A A' a → motive_5 Γ b b' 𝟘 a_1 
+    → motive_5 Γ (A.indEmpty b) (A'.indEmpty b') S (IsEqualTerm.empty_elim_eq a a_1 a_2))
   → (IsEqualTermPiIntroEq : ∀ {n : Nat} {Γ : Ctx n} {A : Tm n} {b b' B : Tm (n + 1)} {A' : Tm n} 
     (a : (Γ ⬝ A) ⊢ b ≡ b' ∶ B), motive_5 (Γ ⬝ A) b b' B a 
     → motive_5 Γ (A.lam b) (A'.lam b') (A.pi B) (IsEqualTerm.pi_intro_eq a))
-  → (IsEqualTermPiElimEq : ∀ {n : Nat} {Γ : Ctx n} {f f' A : Tm n} {B : Tm (n + 1)} {a a' : Tm n} 
-    (a_1 : Γ ⊢ f ≡ f' ∶ A.pi B) (a_2 : Γ ⊢ a ≡ a' ∶ A), motive_5 Γ f f' (A.pi B) a_1 
-    → motive_5 Γ a a' A a_2 → motive_5 Γ (f.app a) (f'.app a') (substitute_zero B a) 
-      (IsEqualTerm.pi_elim_eq a_1 a_2))
+  → (IsEqualTermPiElimEq : ∀ {n : Nat} {Γ : Ctx n} {f f' A : Tm n} {B : Tm (n + 1)} {a a' : Tm n}
+    {S : Tm n} (a_1 : Γ ⊢ f ≡ f' ∶ A.pi B) (a_2 : Γ ⊢ a ≡ a' ∶ A) (a_3 : S = substitute_zero B a),
+    motive_5 Γ f f' (A.pi B) a_1 
+    → motive_5 Γ a a' A a_2 → motive_5 Γ (f.app a) (f'.app a') S (IsEqualTerm.pi_elim_eq a_1 a_2 a_3))
   → (IsEqualTermSigmaIntroEq : ∀ {n : Nat} {Γ : Ctx n} {a a' A b b' : Tm n} {B : Tm (n + 1)} 
     (a_1 : Γ ⊢ a ≡ a' ∶ A) (a_2 : Γ ⊢ b ≡ b' ∶ substitute_zero B a), motive_5 Γ a a' A a_1 
     → motive_5 Γ b b' (substitute_zero B a) a_2 
     → motive_5 Γ (a.pairSigma b) (a'.pairSigma b') (A.sigma B) (IsEqualTerm.sigma_intro_eq a_1 a_2))
   → (IsEqualTermSigmaElimEq :  ∀ {n : Nat} {Γ : Ctx n} {A : Tm n} {B : Tm (n + 1)} {A' : Tm n} 
-    {B' : Tm (n + 1)} {p p' : Tm n} {C C' : Tm (n + 1)} {c c' : Tm (n + 1 + 1)} 
+    {B' : Tm (n + 1)} {p p' : Tm n} {C C' : Tm (n + 1)} {c c' : Tm (n + 1 + 1)} {S : Tm n}
     (a : Γ ⊢ A.sigma B ≡ A'.sigma B' type) (a_1 : Γ ⊢ p ≡ p' ∶ A.sigma B)
     (a_2 : (Γ ⬝ A.sigma B) ⊢ C ≡ C' type)
-    (a_3 : (Γ ⬝ A ⬝ B) ⊢ c ≡ c' ∶ substitute (Subst.weak Weak.id.shift.shift, v(1).pairSigma v(0)) C),
-    motive_4 Γ (A.sigma B) (A'.sigma B') a → motive_5 Γ p p' (A.sigma B) a_1 
-    → motive_4 (Γ ⬝ A.sigma B) C C' a_2 
+    (a_3 : (Γ ⬝ A ⬝ B) ⊢ c ≡ c' ∶ substitute (Subst.weak Weak.id.shift.shift, v(1).pairSigma v(0)) C)
+    (a_4 : S = substitute_zero C p),
+    motive_4 Γ (A.sigma B) (A'.sigma B') a → motive_5 Γ p p' (A.sigma B) a_1
+    → motive_4 (Γ ⬝ A.sigma B) C C' a_2
     → motive_5 (Γ ⬝ A ⬝ B) c c' (substitute (Subst.weak Weak.id.shift.shift, v(1).pairSigma v(0)) C) a_3
-    → motive_5 Γ (A.indSigma B C c p) (A'.indSigma B' C' c' p') (substitute_zero C p)
-      (IsEqualTerm.sigma_elim_eq a a_1 a_2 a_3))
+    → motive_5 Γ (A.indSigma B C c p) (A'.indSigma B' C' c' p') S
+      (IsEqualTerm.sigma_elim_eq a a_1 a_2 a_3 a_4))
   → (IsEqualTermIdenIntroEq : ∀ {n : Nat} {Γ : Ctx n} {A A' a a' : Tm n} 
     (a_1 : Γ ⊢ A ≡ A' type) (a_2 : Γ ⊢ a ≡ a' ∶ A), motive_4 Γ A A' a_1 → motive_5 Γ a a' A a_2 
     → motive_5 Γ (A.refl a) (A'.refl a') (A.iden a a) (IsEqualTerm.iden_intro_eq a_1 a_2))
   → (IsEqualTermIdenElimEq : ∀ {n : Nat} {Γ : Ctx n} {A : Tm n} {B B' : Tm (n + 1 + 1 + 1)} 
-    {b b' : Tm n} {a₁ a₃ A' a₂ a₄ p p' : Tm n}
+    {b b' : Tm n} {a₁ a₃ A' a₂ a₄ p p' : Tm n} {S : Tm n}
     (a : (Γ ⬝ A ⬝ weaken Weak.id.shift A ⬝ (weaken Weak.id.shift.shift A).iden v(1) v(0)) ⊢ B ≡ B' type)
     (a_1 : Γ ⊢ b ≡ b' ∶ substitute (Subst.weak Weak.id, a₁, a₁, .refl A a₁) B)
-    (a_2 : Γ ⊢ A.iden a₁ a₃ ≡ A'.iden a₂ a₄ type) (a_3 : Γ ⊢ p ≡ p' ∶ A.iden a₁ a₃),
+    (a_2 : Γ ⊢ A.iden a₁ a₃ ≡ A'.iden a₂ a₄ type) (a_3 : Γ ⊢ p ≡ p' ∶ A.iden a₁ a₃)
+    (a_4 : S = (substitute (Subst.weak Weak.id, a₁, a₃, p) B)),
     motive_4 (Γ ⬝ A ⬝ weaken Weak.id.shift A ⬝ (weaken Weak.id.shift.shift A).iden v(1) v(0)) B B' a 
     → motive_5 Γ b b' 
       (substitute (Subst.weak Weak.id, a₁, a₁, .refl A a₁) B) a_1
     → motive_4 Γ (A.iden a₁ a₃) (A'.iden a₂ a₄) a_2 → motive_5 Γ p p' (A.iden a₁ a₃) a_3 
-    → motive_5 Γ (A.j B b a₁ a₃ p) (A'.j B' b' a₂ a₄ p') (substitute (Subst.weak Weak.id, a₁, a₃, p) B)
-      (IsEqualTerm.iden_elim_eq a a_1 a_2 a_3))
+    → motive_5 Γ (A.j B b a₁ a₃ p) (A'.j B' b' a₂ a₄ p') S
+      (IsEqualTerm.iden_elim_eq a a_1 a_2 a_3 a_4))
   → (IsEqualTermUnivUnitEq : ∀ {n : Nat} {Γ : Ctx n} 
     (a : Γ ctx), motive_1 Γ a → motive_5 Γ 𝟙 𝟙 𝒰 (IsEqualTerm.univ_unit_eq a))
   → (IsEqualTermUnivEmptyEq : ∀ {n : Nat} {Γ : Ctx n} 
